src/program_proof/buftxn/specs.v
@@ -6,41 +6,51 @@ From Perennial.Helpers Require Import Transitions.
 From Perennial.program_proof Require Import proof_prelude.
 
 From Goose.github_com.mit_pdos.goose_nfsd Require Import addr buftxn.
-From Perennial.program_proof Require Import txn.specs buf.specs.
+From Perennial.program_proof Require Import txn.specs buf.specs addr.specs.
 
 Section heap.
 Context `{!heapG Σ}.
 Context `{!lockG Σ}.
 Context `{!inG Σ (authR (optionUR (exclR boolO)))}.
-Context `{!gen_heapPreG addr txnObject Σ}.
+Context `{!gen_heapPreG addr (sigT (fun K => @bufDataT K)) Σ}.
 
 Implicit Types s : Slice.t.
 Implicit Types (stk:stuckness) (E: coPset).
 
-Definition is_buftxn (buftx : loc) (γT γUnified : gen_heapG addr txnObject Σ) : iProp Σ :=
+Definition is_buftxn (buftx : loc)
+                     (γT : gen_heapG addr (sigT (fun K => @bufDataT K)) Σ)
+                     γUnified : iProp Σ :=
   (
-    ∃ (l : loc) mT bufmap (txid : u64) gBits gInodes gBlocks,
+    ∃ (l : loc) mT (bufmap : loc) (gBufmap : gmap addr buf) (txid : u64),
       buftx ↦[BufTxn.S :: "txn"] #l ∗
       buftx ↦[BufTxn.S :: "bufs"] #bufmap ∗
       buftx ↦[BufTxn.S :: "Id"] #txid ∗
-      is_txn l gBits gInodes gBlocks ∗
-      unify_heaps gBits gInodes gBlocks γUnified ∗
+      is_txn l γUnified ∗
+      is_bufmap bufmap gBufmap ∗
       gen_heap_ctx (hG := γT) mT ∗
-      [∗ map] a ↦ v ∈ mT,
-        ∃ v0,
-          mapsto (hG := γUnified) a 1 v0
+      ( [∗ map] a ↦ b ∈ gBufmap,
+        ⌜ mT !! a = Some (existT _ (bufData b)) ⌝ ) ∗
+      ( [∗ map] a ↦ v ∈ mT,
+        let dirty := match gBufmap !! a with
+                     | None => false
+                     | Some buf => bufDirty buf
+                     end in
+        if dirty then
+          ∃ (v0 : @bufDataT (projT1 v)),
+            mapsto_txn γUnified a v0
+        else
+          mapsto_txn γUnified a (projT2 v) )
   )%I.
 
-Theorem wp_buftxn_Begin l gBits gInodes gBlocks γUnified :
-  {{{ is_txn l gBits gInodes gBlocks ∗
-      unify_heaps gBits gInodes gBlocks γUnified
+Theorem wp_buftxn_Begin l γUnified :
+  {{{ is_txn l γUnified
   }}}
     Begin #l
   {{{ (buftx : loc) γt, RET #buftx;
       is_buftxn buftx γt γUnified
   }}}.
 Proof using gen_heapPreG0.
-  iIntros (Φ) "(Htxn & Hunified) HΦ".
+  iIntros (Φ) "Htxn HΦ".
 
   wp_call.
   wp_apply (wp_MkBufMap with "[$]").
@@ -55,35 +65,204 @@ Proof using gen_heapPreG0.
   iMod (gen_heap_init ∅) as (γt) "Htxctx".
   wp_pures.
   iApply "HΦ".
-  iExists _, _, _, _, _, _, _.
+  iExists _, _, _, _, _.
   iFrame.
-  iApply big_sepM_empty; done.
+  rewrite big_sepM_empty. iFrame.
+  iApply big_sepM_empty. done.
 
   Unshelve. all: eauto. (* XXX why? *)
 Qed.
 
-Theorem wp_BufTxn__ReadBuf__Block buftx γt γUnified a aa v :
+Theorem wp_BufTxn__ReadBuf buftx γt γUnified a sz v :
   {{{
     is_buftxn buftx γt γUnified ∗
-    ⌜ getField_f Addr.S "Sz" a = #(U64 (block_bytes*8)%nat) ⌝ ∗
-    ⌜ getField_f Addr.S "Blkno" a = #aa.(addrBlock) ⌝ ∗
-    ⌜ getField_f Addr.S "Off" a = #aa.(addrOff) ⌝ ∗
-    mapsto (hG := γt) aa 1 (txnBlock v)
+    mapsto (hG := γt) a 1 v ∗
+    ⌜ sz = bufSz (projT1 v) ⌝ ∗
+    ⌜ valid_addr a ⌝
   }}}
-    (* TODO: add size to this spec *)
-    BufTxn__ReadBuf #buftx a
+    BufTxn__ReadBuf #buftx (addr2val a) #sz
   {{{
-    (buf : Slice.t), RET (slice_val buf);
-    is_slice buf u8T 1%Qp (Block_to_vals v) ∗
-    is_buftxn buftx γt γUnified ∗
-    mapsto (hG := γt) aa 1 (txnBlock v)
+    (bufptr : loc) dirty, RET #bufptr;
+    is_buf bufptr a (Build_buf (projT1 v) (projT2 v) dirty) ∗
+    ( ∀ v' dirty',
+      ( ⌜ dirty' = true ∨ (dirty' = dirty ∧ projT2 v = v') ⌝ ∗
+        is_buf bufptr a (Build_buf (projT1 v) v' dirty') ) ==∗
+      ( mapsto (hG := γt) a 1 (existT _ v') ∗
+        is_buftxn buftx γt γUnified ) )
   }}}.
 Proof.
-  iIntros (Φ) "(Htxn & % & % & % & Ha) HΦ".
-  iDestruct "Htxn" as (l mT bufmap txid gBits gInodes gBlocks) "(Hl & Hbufmap & Htxid & Htxn & Hunify & Hγtctx & Hm)".
+  iIntros (Φ) "(Htxn & Ha & -> & %) HΦ".
+  iDestruct "Htxn" as (l mT bufmap gBufmap txid)
+    "(Hl & Hbufmap & Htxid & Htxn & Hisbufmap & Hγtctx & Hbufmapt & Hm)".
   wp_call.
-Admitted.
+  wp_loadField.
+  wp_apply (wp_BufMap__Lookup with "[$Hisbufmap]"); eauto.
+  iIntros (bufptr) "Hbufptr".
+  wp_pures.
+  destruct (gBufmap !! a) eqn:Hbufmap_a.
+  - iDestruct "Hbufptr" as "[Hbufptr Hisbufmap]".
+    iDestruct (is_buf_not_null with "Hbufptr") as %Hbufptr_not_null.
 
+    iDestruct (big_sepM_lookup with "Hbufmapt") as %HmT_a; eauto.
+    iDestruct (gen_heap_valid with "Hγtctx Ha") as %HmT_a2.
+    rewrite HmT_a2 in HmT_a; clear HmT_a2.
+    inversion HmT_a; clear HmT_a; subst.
+    destruct b; rewrite /=.
+
+    wp_if_destruct; try congruence.
+    iApply "HΦ".
+    iFrame "Hbufptr".
+
+    iIntros (v' dirty') "[% Hbufptr]".
+    iDestruct ("Hisbufmap" with "Hbufptr") as "Hisbufmap".
+    intuition idtac.
+    + subst.
+      iMod (gen_heap_update with "Hγtctx Ha") as "[Hγtctx Ha]".
+      iFrame "Ha".
+      iModIntro.
+      iExists _, _, _, _, _.
+      iFrame.
+      iDestruct (big_sepM_lookup with "Hbufmapt") as %HmT_a; eauto.
+      iSplitL "Hbufmapt".
+      {
+        iDestruct (big_sepM_forall with "Hbufmapt") as "Hbufmapt".
+        iApply big_sepM_forall.
+        iIntros (k x).
+        destruct (decide (a = k)).
+        { subst. repeat rewrite lookup_insert.
+          iPureIntro; intros. inversion H0; subst; clear H0.
+          simpl; eauto. }
+        { repeat rewrite -> lookup_insert_ne by eauto.
+          eauto. }
+      }
+
+      iDestruct (big_sepM_delete with "Hm") as "[Hma Hm]"; eauto.
+      iApply big_sepM_insert_delete.
+      iSplitL "Hma".
+      { rewrite lookup_insert. rewrite Hbufmap_a /=.
+        destruct bufDirty; eauto. }
+      iApply (big_sepM_mono with "Hm").
+      iIntros (k x Hkx) "Hk".
+      destruct (decide (a = k)).
+      { subst. rewrite lookup_delete in Hkx. congruence. }
+      rewrite -> lookup_insert_ne by eauto.
+      destruct (gBufmap !! k); eauto.
+
+    + subst.
+      iFrame "Ha".
+      iModIntro.
+      iExists _, _, _, _, _.
+      iFrame.
+      iDestruct (big_sepM_lookup with "Hbufmapt") as %HmT_a; eauto.
+      iSplitL "Hbufmapt".
+      {
+        iDestruct (big_sepM_forall with "Hbufmapt") as "Hbufmapt".
+        iApply big_sepM_forall.
+        iIntros (k x).
+        destruct (decide (a = k)).
+        { subst. repeat rewrite lookup_insert.
+          iPureIntro; intros. inversion H0; subst; clear H0.
+          simpl; eauto. }
+        { repeat rewrite -> lookup_insert_ne by eauto.
+          eauto. }
+      }
+
+      rewrite insert_id; eauto.
+
+  - iDestruct "Hbufptr" as "[-> Hbufptr]".
+    wp_if_destruct.
+    2: congruence.
+
+    wp_loadField.
+    iDestruct (gen_heap_valid with "Hγtctx Ha") as %HmT_a2.
+    iDestruct (big_sepM_lookup_acc with "Hm") as "[Hma Hm]"; eauto.
+    rewrite Hbufmap_a /=.
+
+    iDestruct (is_txn_dup with "Htxn") as "[Htxn Htxn2]".
+    wp_apply (wp_txn_Load with "[$Htxn $Hma]").
+    iIntros (bufptr b) "(Hbuf & % & % & Hma)".
+    wp_pures.
+    iDestruct ("Hm" with "Hma") as "Hm".
+
+    wp_loadField.
+    wp_apply (wp_BufMap__Insert with "[$Hbufptr $Hbuf]").
+    iIntros "Hbufptr".
+
+    wp_loadField.
+    wp_apply (wp_BufMap__Lookup with "[$Hbufptr]"); eauto.
+    iIntros (bufptr2) "Hbufptr2".
+
+    rewrite lookup_insert.
+    iDestruct "Hbufptr2" as "[Hbufptr2 Hisbufmap]".
+
+    destruct b, v. simpl in *.
+    inversion H1; subst.
+    apply eq_sigT_eq_dep in H1.
+    apply Eqdep_dec.eq_dep_eq_dec in H1.
+    2: apply bufDataKind_eq_dec.
+    subst.
+
+    iApply "HΦ".
+    iFrame "Hbufptr2".
+
+    iIntros (v' dirty') "[% Hbufptr]".
+    iDestruct ("Hisbufmap" with "Hbufptr") as "Hisbufmap".
+    intuition idtac.
+    + subst.
+      iMod (gen_heap_update with "Hγtctx Ha") as "[Hγtctx Ha]".
+      iFrame "Ha".
+      iModIntro.
+      iExists _, _, _, _, _.
+      iFrame.
+
+      rewrite insert_insert.
+      iSplitL "Hbufmapt".
+      {
+        iApply (big_sepM_insert); eauto.
+        iSplitR.
+        { rewrite lookup_insert. eauto. }
+        iApply (big_sepM_mono with "Hbufmapt").
+        iIntros (k x0) "% %". iPureIntro.
+        destruct (decide (a = k)).
+        { subst; congruence. }
+        repeat rewrite -> lookup_insert_ne by eauto.
+        eauto.
+      }
+
+      iDestruct (big_sepM_delete with "Hm") as "[Hma Hm]"; eauto.
+      iApply big_sepM_insert_delete.
+      iSplitL "Hma".
+      { rewrite lookup_insert. rewrite Hbufmap_a /=.
+        iExists _; iFrame. }
+      iApply (big_sepM_mono with "Hm").
+      iIntros (k x0 Hkx0) "Hk".
+      destruct (decide (a = k)).
+      { subst. rewrite lookup_delete in Hkx0. congruence. }
+      rewrite -> lookup_insert_ne by eauto.
+      destruct (gBufmap !! k); eauto.
+
+    + subst.
+      iFrame "Ha".
+      iModIntro.
+      iExists _, _, _, _, _.
+      iFrame.
+
+      rewrite insert_insert.
+      iSplitL "Hbufmapt".
+      {
+        iApply (big_sepM_insert); eauto.
+      }
+
+      iApply (big_sepM_mono with "Hm").
+      iIntros (k x0 Hkx0) "Hk".
+      destruct (decide (a = k)).
+      { subst. rewrite lookup_insert. rewrite Hbufmap_a.
+        simpl. eauto. }
+      rewrite -> lookup_insert_ne by eauto.
+      destruct (gBufmap !! k); eauto.
+Qed.
+
+(*
 Theorem wp_BufTxn__OverWrite__Block buftx γt γUnified a aa v0 v (buf : Slice.t) :
   {{{
     is_buftxn buftx γt γUnified ∗
@@ -236,5 +415,6 @@ Proof.
   iApply "Hp".
   iFrame.
 Qed.
+*)
 
 End heap.
